theories/L2_typeStripped/instances.v
@@ -12,26 +12,10 @@ Instance WfL2Term : GoodTerm (Program L2.compile.Term) :=
 
 Instance certiL2 : CerticoqLanguage (Program L2.compile.Term) := {}.
 
-Local Generalizable Variable Lj.
 
-(** TODO : when the dust settles in L1, move this there *)
-Definition translateTo `{CerticoqTranslation (Program L2.compile.Term) Lj}
-  (p:program) : exception Lj :=
-  let l2:= L2.compile.program_Program p in
-  translate (Program L2.compile.Term) Lj l2.
-
-
-Arguments translateTo Lj {H} p.
-
-Definition ctranslateTo {Term Value BigStep WF} 
-  (Lj : @CerticoqLanguage Term Value BigStep WF)
-   `{CerticoqTranslation (Program L2.compile.Term) (cTerm Lj)}
-   : program -> exception (cTerm Lj) :=
-  translateTo (cTerm Lj).
-
-Arguments ctranslateTo {Term0} {Value} {BigStep} {WF} Lj {H} p.
-
-
+Instance certiL1g_to_L2: 
+  CerticoqTotalTranslation (Program L1g.compile.Term) (Program L2.compile.Term) :=
+  stripProgram.
 
 
 
